WIP: MWE List based approach with exchange rules (Alt.lean)

PiLL/PiLL/Alt.lean
@@ -1,4 +1,4 @@
-import Mathlib.Data.Finset.Basic
+import Mathlib.Data.List.Permutation
 import Mathlib.Tactic
 
 abbrev Atom := Nat
@@ -8,15 +8,23 @@ inductive Types : Type where
   | atomDual (a : Atom)
   | one
   | bot
+  | tensor (A B : Types)
+  | parr (A B : Types)
 
 instance : One Types := ⟨Types.one⟩
 instance : Bot Types := ⟨Types.bot⟩
 
+infixr:90 " ⨂ " => Types.tensor
+infixr:90 " ⅋ " => Types.parr
+
+
 def Types.dual : Types → Types
-  | one => bot
-  | bot => one
-  | atom a => atomDual a
-  | atomDual a => atom a
+  | atom a       => atomDual a
+  | atomDual a   => atom a
+  | one          => bot
+  | bot          => one
+  | tensor A B   => parr (dual A) (dual B)
+  | parr A B     => tensor (dual A) (dual B)
 
 postfix:max "ᗮ" => Types.dual
 
@@ -28,40 +36,157 @@ inductive Proc : Type where
   | bot (x : PName) (P : Proc)
   | par (P Q : Proc)
   | cut (x y : PName) (P : Proc)
+  | parr (x y : PName) (P : Proc)
+  | tensor (x y : PName) (P : Proc)
 
-
+notation:80 x "⟦" y "⟧․" P => Proc.tensor x y P
+notation:80 x "⸨" y "⸩․" P => Proc.parr x y P
 notation:80 x "⟦⟧․" P => Proc.one x P
 notation:80 x "⸨⸩․" P => Proc.bot x P
 notation:80 "𝑣⸨"x"," y"⸩"P => Proc.cut x y P
 notation "𝟘" => Proc.nil
-infixr:50 "|ₚ" => Proc.par
+infixr:65 " |ₚ " => Proc.par
 
 abbrev Env := List (PName × Types)
-def Env.mk (x : PName) (A : Types) := [(x, A)]
-notation:80 x "∶" A => Env.mk x A
 
-inductive Split : Env → Env → Env → Prop where
-  | nil : Split ∅ ∅ ∅
+abbrev Env.mk (x : PName) (A : Types) := [(x, A)]
+infixr:86 " ∶ " => Env.mk
 
-  | left (x A Γ Γ₁ Γ₂) :
-      Split Γ Γ₁ Γ₂ →
-      Split ((x, A) :: Γ) ((x, A) :: Γ₁) Γ₂
+abbrev Env.merge (Γ Δ : Env) : Env := Γ ++ Δ
+infixl:85 "‚ " => Env.merge
 
-  | right (x A Γ Γ₁ Γ₂) :
-      Split Γ Γ₁ Γ₂ →
-      Split ((x, A) :: Γ) Γ₁ ((x, A) :: Γ₂)
+abbrev HyperEnv := List Env
 
+abbrev HyperEnv.merge (𝒢 ℋ : HyperEnv) : HyperEnv := 𝒢 ++ ℋ
+infixl:55 " |ₕ " => HyperEnv.merge
 
-inductive Typing : Proc → Env → Prop where
+instance : Coe Env HyperEnv := ⟨fun Γ => ({Γ} : HyperEnv)⟩
+
+inductive Typing : Proc → HyperEnv → Prop where
+  -- | struct {P Q : Proc} {𝒢 ℋ : HyperEnv} :
+  --     Typing P 𝒢 → P ≡ₚ Q → 𝒢.Perm ℋ →
+  --     --------------------------------
+  --     Typing Q ℋ
+
+  | exchange_env {𝒢 : HyperEnv} {Γ Δ : Env} {P : Proc} :
+      Typing P (𝒢 |ₕ Γ) → Γ.Perm Δ →
+      ------------------------------
+      Typing P (𝒢 |ₕ Δ)
+
+  | exchange_hyper {𝒢 ℋ : HyperEnv} {P : Proc} :
+      Typing P 𝒢 → 𝒢.Perm ℋ →
+      ------------------------
+      Typing P ℋ
+
   | mix₀ :
-    Typing 𝟘 ∅
+      Typing 𝟘 ∅
 
-  | mix {P Q : Proc} {Γ Γ₁ Γ₂ : Env} :
-    Split Γ Γ₁ Γ₂ → Typing P Γ₁ → Typing Q Γ₂ →
-    Typing (P |ₚ Q) Γ
+  | mix {𝒢 ℋ : HyperEnv} {P Q : Proc} :
+      Typing P 𝒢 → Typing Q ℋ →
+      --------------------------
+      Typing (P |ₚ Q) (𝒢 |ₕ ℋ)
 
-  | one {x : PName} {P : Proc} :
-    Typing (x⟦⟧․P) (x ∶ 1)
+  | one {P : Proc} {x : PName} :
+      Typing P ∅ →
+      ----------------------
+      Typing (x⟦⟧․P) (x ∶ 1)
+
+  | bot {Γ : Env} {P : Proc} {x : PName} :
+      Typing P Γ →
+      -------------------------
+      Typing (x⸨⸩․P) (Γ‚ x ∶ ⊥)
+
+  | cut {𝒢 : HyperEnv} {Γ Δ : Env} {P : Proc} {x y : PName} {A : Types} :
+      Typing P (𝒢 |ₕ Γ‚ x ∶ A |ₕ Δ‚ y ∶ Aᗮ) →
+      -------------------------------------------
+      Typing (𝑣⸨x, y⸩ P) (𝒢 |ₕ Γ‚ Δ)
+
+  | tensor {Γ Δ : Env} {P : Proc} {x y : PName} {B A : Types} :
+      Typing P (Γ‚ y ∶ A |ₕ Δ‚ x ∶ B) →
+      ---------------------------------
+      Typing (x⟦y⟧․P) (Γ‚ Δ‚ x ∶ A ⨂ B)
+
+  | parr {Γ : Env} {P : Proc} {x y : PName} {A B : Types} :
+      Typing P (Γ‚ y ∶ A‚ x ∶ B) →
+      ------------------------------
+      Typing (x⸨y⸩․P) (Γ‚ x ∶ A ⅋ B)
+
+notation:65 "⊢ " P " ∷ " 𝒢 => Typing P 𝒢
+
+
+
+
+lemma Env.merge_unitL (Γ : Env) : ∅‚ Γ = Γ := by simp
+
+lemma Env.merge_unitR (Γ : Env) : Γ‚ ∅ = Γ := by simp
+
+lemma Env.merge_comm (Γ Δ : Env) : List.Perm (Γ‚ Δ) (Δ‚ Γ) := by
+  exact List.perm_append_comm
+
+lemma Env.merge_assoc (Γ Δ Ξ : Env) : Γ‚ Δ‚ Ξ = Γ‚ (Δ‚ Ξ) := by
+  simp [Env.merge]
+
+lemma Env.merge_rotate_left (Γ : Env) (x : PName × Types) :
+  (x :: Γ).Perm (Γ‚ [x]) := by
+  symm ; apply List.perm_append_singleton
+
+lemma Env.merge_swap (Γ : Env) (x y : PName × Types) :
+  List.Perm (x :: y :: Γ) (y :: x :: Γ) := by
+  symm ; simpa using List.Perm.swap x y Γ
+
+lemma HyperEnv.merge_unitL (𝒢 : HyperEnv) : ∅ |ₕ 𝒢 = 𝒢 := by simp
+
+lemma HyperEnv.merge_unitR (𝒢 : HyperEnv) : 𝒢 |ₕ ∅ = 𝒢 := by simp
+
+lemma HyperEnv.merge_comm (𝒢 ℋ : HyperEnv) : List.Perm (𝒢 |ₕ ℋ) (ℋ |ₕ 𝒢) := by
+  exact List.perm_append_comm
+
+lemma HyperEnv.merge_assoc (𝒢 ℋ ℐ : HyperEnv) : 𝒢 |ₕ ℋ |ₕ ℐ = 𝒢 |ₕ (ℋ |ₕ ℐ) := by
+  simp [HyperEnv.merge]
+
+lemma HyperEnv.rotate_left (𝒢 : HyperEnv) (Γ : Env) :
+  (Γ :: 𝒢).Perm (𝒢 ++ Γ) := by
+  symm ; apply List.perm_append_singleton
+
+lemma HyperEnv.merge_swap (𝒢 : HyperEnv) (Γ Δ : Env) :
+  List.Perm (Γ :: Δ :: 𝒢) (Δ :: Γ :: 𝒢) := by
+  symm ; simpa using List.Perm.swap Γ Δ 𝒢
+
+
+lemma Typing.env_comm {P : Proc} {𝒢 : HyperEnv} {Γ Δ : Env} :
+  (⊢ P ∷ 𝒢 |ₕ Γ‚ Δ) → (⊢ P ∷ 𝒢 |ₕ Δ‚ Γ) :=
+  fun h => Typing.exchange_env h (Env.merge_comm _ _)
+
+lemma Typing.env_rotate {P : Proc} {𝒢 : HyperEnv} {Γ : Env} {x : PName × Types} :
+  (⊢ P ∷ 𝒢 |ₕ Γ‚ [x]) → (⊢ P ∷ 𝒢 |ₕ {x :: Γ}) :=
+  fun h => Typing.exchange_env h (by symm ; apply Env.merge_rotate_left _ _)
+
+lemma Typing.hyper_comm {P : Proc} {𝒢 ℋ : HyperEnv} :
+  (⊢ P ∷ 𝒢 |ₕ ℋ) → (⊢ P ∷ ℋ |ₕ 𝒢) :=
+  fun h => Typing.exchange_hyper h (HyperEnv.merge_comm _ _)
+
+
+
+
+example : ⊢ ((10⟦⟧․𝟘) |ₚ (40⸨⸩․30⸨⸩․20⟦⟧․𝟘)) ∷
+  ((40 ∶ ⊥)‚ (30 ∶ ⊥)‚ 20 ∶ 1) |ₕ (10 ∶ 1) := by
+  apply Typing.hyper_comm
+  · apply Typing.mix
+    · apply Typing.one
+      apply Typing.mix₀
+    · apply Typing.env_rotate (𝒢 := ∅)
+      · apply Typing.bot
+        apply Typing.exchange_env (𝒢 := ∅)
+          (Γ := ((20 ∶ 1)‚ 30∶ ⊥))
+        · apply Typing.bot
+          · apply Typing.one
+            apply Typing.mix₀
+        · exact Env.merge_comm _ _
+
+
+
+
+
 
 
 inductive Lbl : Type where
@@ -69,30 +194,6 @@ inductive Lbl : Type where
   | bot (x : PName)
 
 inductive ProcStep : Proc → Lbl → Proc → Prop where
-  | one {x : PName} {P : Proc} :
-    ProcStep (x⟦⟧․P) (Lbl.one x) P
 
-  | par₁ {P P' Q : Proc} {l : Lbl}:
-    ProcStep P l P' →
-    ProcStep (P |ₚ Q) l (P' |ₚ Q)
-
-  | res
-      {P P' : Proc} {x y : PName} {l : Lbl} :
-      ProcStep P l P' →
-      ProcStep (𝑣⸨x, y⸩ P) (l) (𝑣⸨x, y⸩ P')
 
 inductive EnvStep : Env → Lbl → Env → Prop where
-  | one {x : PName} :
-    EnvStep (x ∶ 1) (Lbl.one x) ∅
-
- | par₁
-    {𝒢 𝒢' Γ Γ' Δ : Env} {l : Lbl} :
-    Split 𝒢 Γ Δ → EnvStep Γ l Γ' →
-    Split 𝒢' Γ' Δ → EnvStep 𝒢 l 𝒢'
-
-  | res {𝒢 𝒢' E𝒢'Γx 𝒢' EΓx Γ EΔy Δ : Env} {x y : PName} {A : Types} {l : Lbl}:
-    Split EΓx Γ (x ∶ Aᗮ) → Split EΔy (Δ) (y ∶ A) → Split E𝒢'Γx 𝒢' EΓx →
-    Split 𝒢 E𝒢'Γx EΔy →
-
-
-    EnvStep 𝒢 l 𝒢' →
